\documentclass[12pt, a4 paper]{article}
% Set target color model to RGB
\usepackage[inner=2.0cm,outer=2.0cm,top=2.5cm,bottom=2.5cm]{geometry}
\usepackage{setspace}
\usepackage[rgb]{xcolor}
\usepackage{environ}
\usepackage{verbatim}
\usepackage{subcaption}
\usepackage{outlines}
\usepackage{amsgen,amsmath,amstext,amsbsy,amsopn,tikz,amssymb,tkz-linknodes}
\usepackage{fancyhdr}
\usepackage{pgfplots}
\usepackage{mathtools}
\usepackage[colorlinks=true, urlcolor=blue,  linkcolor=blue, citecolor=blue]{hyperref}
\usepackage[colorinlistoftodos]{todonotes}
\usepackage{rotating}

\linespread{1.6} % Double Line Spacing
\usetikzlibrary{arrows.meta,intersections,calc}


\hypersetup{%
pdfauthor={Vignesh Ravibaskar},%
pdfcreator={PDFLaTeX},%
pdfproducer={PDFLaTeX},%
}
\usepackage{enumitem}
\setlist[enumerate,1]{label=\textbf{\arabic*}}
\setlist[enumerate,2]{label=\textbf{({\alph*})}}
\setlist[enumerate,3]{label=\textbf{({\roman*})}}

\title{Functions}
\author{Derek, Vignesh}
\date{2020}

\newcommand{\comm}[1]{}
\NewEnviron{answer}{\vspace{3mm} \\ \color{blue} {\BODY} \color{black}}
% \NewEnviron{answer}{\color{blue} \comm{\BODY} \color{black}} % Use this method to hide all answers

\begin{document}

\maketitle

\textbf{FUNCTIONS [60 Marks]}
\begin{outline}[enumerate]
 \1 The function f is defined by \[\textrm{f}:x \mapsto \left|\ln{(3x)+1}\right|, x>a.\] %Question 1

 \2 Find the smallest value of \(a\) such that \textrm{f}\(^{-1}\) exists.\hfill[1]
 \begin{answer}
  Solving \(\textrm{f}(x)=0\), we get \(x=\dfrac{1}{3\mathrm{e}}\). Thus, the smallest value of \(a\), \(a_{\min}=\dfrac{1}{3\mathrm{e}}\)
 \end{answer}

 \2 Using the domain of f found in \textbf{(a)}, sketch the graph of \(y=\textrm{f}(x)\) and \(y=\textrm{f}^{-1}(x)\) on the same diagram. \hfill[4]
 \begin{answer}
  To get \(\textrm{f}^{-1}(x)\), we make \(y\) the subject of the equation \(x=|\ln{(3y)+1}|\) so we get \(\textrm{f}^{-1}(x)=\dfrac{\mathrm{e}^{x-1}}{3}\) \\
  \vspace{3mm}
  \color{black}
  \begin{tikzpicture}
   \begin{axis}[
     axis lines = center,
     xlabel = \(x\),
     ylabel = \(y\),
     xmin = 0, xmax=5,
     ymin = 0, ymax=5,
     legend pos=outer north east
    ]
    \addplot [
     domain=1/(3*e):5,
     samples=100,
     color=blue,
    ]
    {abs(ln(3*x)+1)};
    \addlegendentry{\)\textrm{f}(x)=\left|\ln{(3x)+1}\right|\)}
    \addplot [
     domain=0:5,
     samples=100,
     color=red,
    ]
    {(e^(x-1))/3};
    \addlegendentry{\)\textrm{f}^{-1}(x)=\frac{\mathrm{e}^{x-1}}{3}\)}
   \end{axis}
  \end{tikzpicture}
 \end{answer}


 \1 The function f is defined by \[\textrm{f}:x \mapsto \sqrt{a^2-x^2}+k,\;0< x <a.\] %Question 2

 \2 Given that f is \emph{self-inverse}, meaning that \(\textrm{f}(x)=\textrm{f}^{-1}(x)\), state the conditions that must be fulfilled by \(a\) and \(k\). \hfill[2]
 \begin{answer}
  Let us make \(x\) the subject of the equation \(y=\sqrt{a^2-x^2}+k\)
  \begin{align*}
   y         & =\sqrt{a^2-x^2}+k      \\
   {(y-k)}^2 & = a^2-x^2              \\
   x         & = \sqrt{a^2-{(y-k)}^2}
  \end{align*}
  It is evident that the equation is \emph{self-inverse} for \(a\in\mathbb{R}^+, k=0\)
 \end{answer}

 \2 Hence, find the exact value of \(x\) such that \(\textrm{f}^{-1}\textrm{f}^{-1}(x)=\textrm{f}\textrm{f}\textrm{f}(x)\).\hfill[3]
 \begin{answer}
  Since \(\textrm{f}(x)=\textrm{f}^{-1}(x)\), \(\textrm{f}^{-1}\textrm{f}^{-1}(x)=\textrm{f}\textrm{f}\textrm{f}(x)\) can be found by solving \(x=\mathrm{f}x\)
  \begin{align*}
   x          & =\sqrt{a^2-x^2}       \\
   \implies x & =\sqrt{\frac{a^2}{2}}
  \end{align*}
 \end{answer}

 \1 The function f is defined by \[\textrm{f}:x \mapsto \frac{1}{2}\sqrt{4-x^2},\;0\leq x \leq2.\] %Question 3

 \2 Find \(\textrm{f}^{-1}(x)\) and state the domain and range of \(\textrm{f}^{-1}\).\hfill[2]
 \begin{answer}
  To find \(\textrm{f}^{-1}(x)\), let us make \(x\) the subject of \(y=\frac{1}{2}\sqrt{4-x^2}\)
  \begin{align*}
   y & =\frac{1}{2}\sqrt{4-x^2}   \\
     & \implies 4y^2=4-x^2        \\
     & \implies x = 2\sqrt{1-y^2}
  \end{align*}
  Thus, \(\textrm{f}^{-1}(x)=2\sqrt{1-x^2}\). Further, we know that D\)_{\textrm{f}^{-1}} = \textrm{R}_\textrm{f} = [0,1], \textrm{R}_{\textrm{f}^{-1}} = \textrm{D}_\textrm{f} = [0,2]\)
 \end{answer}

 \2 State the domains and ranges of \(\textrm{f}\textrm{f}^{-1}\) and \(\textrm{f}^{-1}\textrm{f}\).\hfill[2]
 \begin{answer}
  D\)_{\textrm{f}\textrm{f}^{-1}}\) = D\)_{\textrm{f}^{-1}}\) = \([0,1]\), R\)_{\textrm{f}\textrm{f}^{-1}} = [0,1]\) \\
  D\)_{\textrm{f}^{-1}\textrm{f}}\) = D\)_{\textrm{f}}\) = \([0,2]\), R\)_{\textrm{f}^{-1}\textrm{f}}\)= \([0,2]\)
 \end{answer}

 \2 State the set of values of \(x\) for which \(\textrm{f}\textrm{f}^{-1}(x)=\textrm{f}^{-1}\textrm{f}(x)\).\hfill[1]
 \begin{answer}
  The set of values is \([0,1] \cap [0,2] = [0,1]\)
 \end{answer}

 \2 Find the exact solution of \(\textrm{f}\textrm{f}^{-1}\textrm{f}(x)=\frac{1}{2}\).\hfill[2]
 \begin{answer}
  Since \(\textrm{f}^{-1}\textrm{f}(x)=x\), we can solve for \(x\) in \(\textrm{f}(x)=\frac{1}{2}\) which is equivalent to \(\textrm{f}^{-1}(\frac{1}{2})=\sqrt{3}\)
 \end{answer}

 \1 The function f is defined by \[\textrm{f}(x)=\frac{1}{1-x},\;x\in \mathbb{R}\]

 \2 Show that \(\textrm{f}\textrm{f}\textrm{f}(x)=x\).\hfill[2]
 \begin{answer}
  \begin{align*}
   \textrm{f}\textrm{f}\textrm{f}(x) & =\textrm{f}\textrm{f}\left(\frac{1}{1-x}\right)    \\
                                     & = \textrm{f}\left(\frac{1}{1-\frac{1}{1-x}}\right) \\
                                     & = \textrm{f}\left(\frac{1-x}{1-x-1}\right)         \\
                                     & = \textrm{f}\left(-\frac{1}{x}+1\right)            \\
                                     & = -\frac{1}{(\frac{1}{1-x})}+1                     \\
                                     & = x\;\textrm{(shown)}
  \end{align*}
 \end{answer}
 \2 Show that \(\textrm{f}^{-1}\textrm{f}^{-1}(x)=\textrm{f}(x)\).\hfill[2]
 \begin{answer}
  To find \(\textrm{f}^{-1}(x)\), let us make \(x\) the subject of \(y=\frac{1}{1-x}\)
  \begin{align*}
   y   & = \frac{1}{1-x}   \\
   1-x & = \frac{1}{y}     \\
   x   & = 1 - \frac{1}{y} \\
  \end{align*}
  Therefore, \(\textrm{f}^{-1}(x) = 1 - \frac{1}{x}\).
 \end{answer}
 \begin{answer}
  We now simplify the composite function \(\textrm{f}^{-1}\textrm{f}^{-1}(x)\)
  \begin{align*}
   \textrm{f}^{-1}\textrm{f}^{-1}(x) & = \textrm{f}^{-1}(1 - \frac{1}{x}) \\
                                     & = 1 - \frac{1}{1 - \frac{1}{x}}    \\
                                     & = 1 - \frac{x}{x-1}                \\
                                     & = \frac{x-1-x}{x-1}                \\
                                     & = \frac{1}{1-x}                    \\
                                     & = \textrm{f}(x)\;\textrm{(shown)}
  \end{align*}
 \end{answer}
 \2 Hence, find the exact value(s) of a such that \(\textrm{f}(\textrm{f}\textrm{f}\textrm{f}(a)+\textrm{f}\textrm{f}(a)+\textrm{f}(a))=\textrm{f}^{-1}(a)\). \hfill[4]
 \begin{answer}
  We will apply \(\textrm{f}^{-1}\) on both sides so the RHS of the equation becomes \(\textrm{f}^{-1}\textrm{f}^{-1}(a)\) to utilise our result in \textbf{(b)}. We then simplify the composite functions \(\textrm{f}\textrm{f}\textrm{f}\) and \(\textrm{f}\textrm{f}\) using our working in \textbf{(a)}.
  \begin{align*}
   \textrm{f}(\textrm{f}\textrm{f}\textrm{f}(a)+\textrm{f}\textrm{f}(a)+\textrm{f}(a)) & =\textrm{f}^{-1}(a)                \\
   \textrm{f}\textrm{f}\textrm{f}(a)+\textrm{f}\textrm{f}(a)+\textrm{f}(a)             & =\textrm{f}^{-1}\textrm{f}^{-1}(a) \\
   a-\frac{1}{a}+\textrm{f}(a)                                                         & =\textrm{f}(a)                     \\
   a^2-1                                                                               & =0                                 \\
   \therefore a                                                                        & =\pm 1
  \end{align*}
 \end{answer}
 %Question 4

 \1 The function f is defined by
 \[\textrm{f}(x)=
  \begin{cases}
   -\dfrac{1}{1+x} & \textrm{for }-1<x<1, \\
   \frac{1}{2}x-1  & \textrm{for }x\geq1.
  \end{cases}
 \] %Question 5

 \2 Sketch the graph of f. Hence, show that f is one-one. \hfill[3]
 \begin{answer}
  \vspace{3mm}
  \color{black}
  \begin{tikzpicture}
   \begin{axis}[
     axis lines = center,
     xlabel = \(x\),
     ylabel = \(y\),
     xmin = -2, xmax=5,
     ymin=-5, ymax = 2,
     legend pos=outer north east
    ]
    \addplot [
     domain=-1:1,
     samples=100,
     color=blue,
    ]
    {-1/(1+x)};
    \addplot [
     domain=1:5,
     samples=100,
     color=blue,
    ]
    {0.5*x-1};
    \addlegendentry{\)\textrm{f}(x)\)};
    \node[label={270:{\)(1,-\frac{1}{2})\)}},circle,fill,inner sep=2pt] at (axis cs:1,-0.5) {};
    \draw[dashed] ({axis cs:-1,0}|-{rel axis cs:0,0}) -- ({axis cs:-1,0}|-{rel axis cs:0,1});
   \end{axis}
  \end{tikzpicture}
  \color{blue}
  The graph of \(y=a\) cuts \(\textrm{f}(x)\) at one and only one point \(\forall a\in\mathbb{R}\implies \) the function is one-one.
 \end{answer}

 \2 Find \(\textrm{f}^{-1}\). \hfill[2]
 \begin{answer}
  Making \(x\) the subject for both \(y=-\dfrac{1}{1+x}\) and \(y=\dfrac{1}{2}x-1\):
  \begin{align*}
   \implies x=-\frac{1}{y}-1 \quad\textrm{and}\quad x=2(y+1) \\
   \therefore\textrm{f}^{-1}(x)=
   \begin{cases}
    -\frac{1}{x}-1 & \textrm{for }x<-\frac{1}{2},    \\
    2(x+1)         & \textrm{for }x\geq-\frac{1}{2}.
   \end{cases}
  \end{align*}
 \end{answer}

 \1 The function f is defined by \[\textrm{f}:x \mapsto \frac{x^2+1}{x-1},\;x>a.\] %Question 6

 \2 Given that f is one-one, state the exact value of \(a\). \hfill[2]
 \begin{answer}
  By plotting the result on a G.C., we can see that \(a\) must be the \(x\)-coordinate of the minimum point of the curve. To obtain stationary points, we have to differentiate \(\textrm{f}(x)\) with respect to \(x\).
  \begin{align*}
   \textrm{f}(x)  & =x+1+\frac{2}{x-1}                                         \\
   \textrm{f}'(x) & =1-\frac{2}{{(x-1)}^2}=0 \textrm{   for stationary points} \\
                  & \implies {(x-1)}^2=2                                       \\
                  & x=1\pm \sqrt{2}
  \end{align*}
  From the G.C., we can observe that the \(x\)-coordinate of the minimum point is greater than that of the maximum point. Therefore, \(a=1+\sqrt{2}\).
 \end{answer}
 \2 Find \(\textrm{f}^{-1}(x)\) and state the domain and range of \(\textrm{f}^{-1}\).\hfill[5]
 \begin{answer}
  To find \(\textrm{f}^{-1}(x)\), let us make \(x\) the subject of \(y=\frac{x^2+1}{x-1}\).
  \begin{align*}
   y          & =\frac{x^2+1}{x-1}               \\
   y(x-1)     & =x^2+1                           \\
   x^2-yx+y+1 & =0                               \\
   x          & = \frac{y\pm \sqrt{y^2-4y-4}}{2}
  \end{align*}
  To eliminate the \(\pm \), we must find the range of values of \(y\), or \(\textrm{R}_{\textrm{f}}\). From the G.C. we know that the \(y\)-coordinate of the minimum point is the lower limit of \(\textrm{R}_{\textrm{f}}\).
  \begin{align*}
   \textrm{Substituting }x=1+\sqrt{2},\; y & =\frac{{(1+\sqrt{2})}^2+1}{1+\sqrt{2}-1} \\
                                           & = \frac{(4+2\sqrt{2})}{\sqrt{2}}         \\
                                           & = 2\sqrt{2}+2
  \end{align*}
  Since \(y>2\sqrt{2}+2\), \(\sqrt{y^2-4y-4}>\sqrt{{(2\sqrt{2}+2)}^2-4(2\sqrt{2}+2)-4}=0\).\\
  It follows that \(\frac{y-\sqrt{y^2-4y-4}}{2}<1+\sqrt{2}\).\\
  However, \(x \in (1+\sqrt{2},\infty)\), so we can only take \(\frac{y+\sqrt{y^2-4y-4}}{2}\).\\
  \(\therefore \;\textrm{f}^{-1}(x)=\frac{x+\sqrt{x^2-4x-4}}{2}\).\\
  As found earlier, \(\textrm{D}_{\textrm{f}^{-1}}=\textrm{R}_{\textrm{f}}=(2+2\sqrt{2},\infty)\) and \(\textrm{R}_{\textrm{f}^{-1}}=\textrm{D}_{\textrm{f}}=(1+\sqrt{2},\infty)\)
 \end{answer}
 \1 Functions f and g are defined as follows:
 \begin{align*}
   & \textrm{f}(x)=\frac{1}{2}\mathrm{e}^{1-x},\;x\geq0, \\
   & \textrm{g}(x)=1-\ln{(x)},\;0<x\leq{\mathrm{e}}.
 \end{align*} %Question 7

 \2 Show that both fg and gf exist.\hfill[3]
 \begin{answer}
  \vspace{3mm}
  \color{black}
  \begin{tikzpicture}
   \begin{axis}[
     axis lines = center,
     xlabel = \(x\),
     ylabel = \(y\),
     xmin = 0, xmax=4,
     ymin=0, ymax = 4,
     legend pos=outer north east
    ]
    \addplot [
     domain=0:4,
     samples=100,
     color=blue,
    ]
    {0.5*e^(1-x)};
    \addlegendentry{\(\textrm{f}(x)\)};
    \addplot [
     domain=0:e,
     samples=100,
     color=red,
    ]
    {1-ln(x)};
    \addlegendentry{\(\textrm{g}(x)\)};
   \end{axis}
  \end{tikzpicture}
  \color{blue}
  R\(_\textrm{g} = \mathbb{R}^+_0 =\) D\(_\textrm{f}\implies \) fg exists \\
  R\(_\textrm{f} = \left(0,\frac{1}{2}\mathrm{e}\right] \subset (0,\mathrm{e}] \) = D\(_\textrm{g}\implies \) gf exists
 \end{answer}

 \2 By finding expressions for fg and gf, find the exact solution of \(\textrm{fg}(2)=\textrm{gf}(\ln{(x)})\).\hfill[3]\\
 \begin{answer}
  fg\((x)=\frac{1}{2}\mathrm{e}^{1-(1-\ln{x})} = \frac{1}{2}x\) \\
  gf\((x) = 1-\ln{(\frac{1}{2}\mathrm{e}^{1-x})} = 1-\ln{(\frac{1}{2}\cdot \mathrm{e} \cdot \mathrm{e}^{-x})} = 1-(-\ln2+1-x) = x+\ln2\)
  \begin{align*}
   \textrm{gf}(\ln x) & = \ln2x              \\
                      & = \textrm{fg}(2) = 1 \\
   \implies x=\frac{\mathrm{e}}{2}
  \end{align*}
 \end{answer}

 \1 The functions f and g are defined by: \[\textrm{f}(x)=
  \begin{cases}
   2\sqrt{x-2}           & \textrm{for }2\leq x<6, \\
   6-\sqrt{\frac{2}{3}x} & \textrm{for }x\geq6.
  \end{cases}
  \quad\textrm{and}\quad \textrm{g}(x)=x^2,\;x\in \mathbb{R}.\]
 %Question 8

 \2 Show that gf exists. \hfill[2]
 \begin{answer}
  Notice that the maximum value of \(\textrm{(x)}\) is equal to 4 when \(x=6\).\\
  R\(_\textrm{f} = (-\infty,4] \subset \mathbb{R} = \textrm{D}_{\textrm{g}}\implies \) gf exists.
 \end{answer}
 \2 Find the exact value of \(\textrm{gf}(4)\).\hfill[2]
 \begin{answer}
  Since \(4\in [2,6)\) for which \(\textrm{f}(x)=2\sqrt{x-2}\),
  \begin{align*}
   \textrm{gf}(x) & = \textrm{g}(2\sqrt{x-2}) \\
                  & = {(2\sqrt{x-2})}^2       \\
                  & = 4(x-2)
  \end{align*}
  \(\therefore \textrm{gf}(4)=4(2)=8\)
 \end{answer}
 \2 Find the exact value of \(x\) such that \(\textrm{gf}(x)=5\).\hfill[2]
 \begin{answer}
  We have already found \(\textrm{gf}(x)\) in terms of \(x\) in the previous answer. All we need to do is to equate this expression to 5.
  \begin{align*}
   \textrm{gf}(x) = 4(x-2) & = 5           \\
   x                       & =\frac{13}{4}
  \end{align*}
 \end{answer}
 \1 The function h is defined by: \[\textrm{h}(n)=
  \begin{cases}
   n(\textrm{h}(n-1)) & \textrm{for }n>1, \\
   1                  & \textrm{for }n=1.
  \end{cases}\]
 where \(n \in \mathbb{Z}^+\).

 \2 State the values of \(\textrm{h}(2)\), \(\textrm{h}(3)\) and \(\textrm{h}(4)\).\hfill[1]
 \begin{answer}
  \(h(2)=2(h(1))=2, h(3)=3(h(2))=6, h(4)=4(h(3))=24\)
 \end{answer}

 \2 Deduce the use of function h.\hfill[1]
 \begin{answer}
  \(h(n)=n! \)
 \end{answer}

 \2 Evaluate \(\dfrac{\textrm{h}(40)}{\textrm{h}(10)\textrm{h}(30)}\). \hfill[2]
 \begin{answer}
  Notice that this is just \(\left(\begin{smallmatrix}40\\30\end{smallmatrix}\right)\).
  \begin{align*}
   \frac{\textrm{h}(40)}{\textrm{h}(10)\textrm{h}(30)} = \frac{40!}{10!30!} = 847660528
  \end{align*}
 \end{answer}

 \1 The function f has an inverse and is such that \[\textrm{f}:x^2+3 \mapsto x,\;x>0.\]

 \2 Find \(\textrm{f}(x)\), and write down its domain and range.\hfill[3]
 \begin{answer}
  Making \(x\) the subject of \(y=x^2+3\), we get \(x=\pm\sqrt{y-3}\). Since D\(_{\textrm{f}^{-1}} = \mathbb{R}^+\), \(f(x) = \sqrt{x-3}\) and R\(_\textrm{f}=\mathbb{R}^+\) and D\(_\textrm{f}=(3,\infty)\)
 \end{answer}

 \2 The function g is such that \(\textrm{g}(3x+2)=\textrm{f}(x)\).\\ Find \(\textrm{g}(x)\). State its domain and range.\hfill[4]
 \begin{answer}
  Given that \(\textrm{g}(3x+2)\) has exactly the same graph as \(\textrm{f}(x)\), we can manipulate the terms within the brackets.\\
  Subtracting 2 units on  both sides, \(\textrm{g}(3x)=\textrm{f}(x-2)\).\\
  Dividing by 3 on both sides,
  \begin{align*}
   \textrm{g}(x) & =\textrm{f}\left(\frac{x-2}{3}\right) \\
                 & = \sqrt{\frac{x-2}{3}-3}              \\
                 & = \sqrt{\frac{x-11}{3}}
  \end{align*}
  To find the domain of g, we perform the same transformations.\\
  Since \(x>3\), \(3x+2>11\). D\(_{\textrm{g}}=(11,\infty)\) \newline
  The range of g is clearly R\(_\textrm{g}=\mathbb{R}^+\).\newline \newline
  Alternatively, one can deduce this using the fact that \(\textrm{g}(x)\) is a square root function, which means it cannot take negative values.
 \end{answer}

 \1 Decomposing \(\dfrac{12x^2+12x}{{(2x+1)}^2}\) into the form \(A + \dfrac{B}{{(2x+1)}^2}\), find a series of transformations that gives \(\dfrac{12x^2+12x}{{(2x+1)}^2}\) from \(\dfrac{3}{x^2}\)
 \begin{answer}
  By inspection, it is evident that \(A = \frac{12x^2}{4x^2} = 3\). Now we shall solve for \(B\)
  \begin{align*}
   B                                     & = 12x^2 + 12x - 3{(2x+1)}^2     \\
                                         & = 12x^2 + 12x - 3(4x^2 + 4x -3) \\
                                         & = -3                            \\
   \implies \frac{12x^2+12x}{{(2x+1)}^2} & = 3-\frac{3}{{2x+1)}^2}
  \end{align*}

  We want to transform \(\frac{3}{x^2}\) into \(3 - \frac{3}{{(2x+1)}^2}\). Beginning with \(y=\frac{3}{x^2}\):\\
  1. Reflect the graph about the y-axis
  \begin{align*}
   y =- \frac{3}{x^2}
  \end{align*}
  2. Shift the graph up by 3 units along the \(+y\)-axis: Replace \(y\) with \(y-3\)
  \begin{align*}
   (y-3) & = -\frac{3}{x^2}    \\
   y     & = 3 - \frac{3}{x^2}
  \end{align*}
  3a. Shift the graph by 1 unit against the \(+x\)-axis: Replace \(x\) with \(x+1\)
  \begin{align*}
   y & = 3 - \frac{3}{{(x+1)}^2}
  \end{align*}
  4a. Scale the graph by \(2\times \) along the \(x\)-axis: Replace \(x\) with \(2x\)
  \begin{align*}
   y & = 3 - \frac{3}{{(2x+1)}^2}     \\
     & =\dfrac{12x^2+12x}{{(2x+1)}^2}
  \end{align*}
  \color{red}\textbf{OR}\color{blue} \\
  3b.  Scale the graph by \(2\times \) along the \(x\)-axis: Replace \(x\) with \(2x\)
  \begin{align*}
   y & = 3 - \frac{3}{{(2x)}^2}
  \end{align*}
  4b. Shift the graph by 0.5 unit against the \(+x\)-axis: Replace \(x\) with \(x+\frac{1}{2}\)
  \begin{align*}
   y & = 3 - \frac{3}{{(2(x+\frac{1}{2}))}^2} \\
   y & = 3 - \frac{3}{{(2x+1)}^2}             \\
     & = \dfrac{12x^2+12x}{{(2x+1)}^2}
  \end{align*}

 \end{answer}

\end{outline}

\end{document}
